src/Extraction/Extract.v
@@ -1,0 +1,9 @@
+From Stdlib Require Import String ZArith List Extraction.
+From Stdlib Require Import ExtrOcamlBasic ExtrOcamlNativeString ExtrOcamlZBigInt.
+From MlirSem Require Import Syntax.AST.
+
+Extraction Language OCaml.
+Set Extraction AccessOpaque.
+Set Extraction Output Directory ".".
+
+Extraction "AST.ml" MlirSem.Syntax.AST.mlir_program.
