test/simple_arith.mlir
@@ -1,0 +1,4 @@
+func.func @main() -> (i32) {
+  %0 = arith.constant 42 : i32
+  func.return %0 : i32
+}
